DeBruijnSSA/BinSyntax/Typing/Region/Structural.lean
@@ -1,0 +1,182 @@
+import DeBruijnSSA.BinSyntax.Typing.Ctx
+import DeBruijnSSA.BinSyntax.Typing.LCtx
+import DeBruijnSSA.BinSyntax.Typing.Term.Basic
+import DeBruijnSSA.BinSyntax.Typing.Region.LSubst
+import DeBruijnSSA.BinSyntax.Typing.Region.Compose
+
+namespace BinSyntax
+
+namespace Term
+
+variable
+  [Φ: EffInstSet φ (Ty α) ε] [PartialOrder α] [PartialOrder ε] [OrderBot ε]
+  {Γ Δ : Ctx α ε} {σ : Region.Subst φ}
+
+def pack0 (ℓ : ℕ) : Term φ := inr^[ℓ] (inl (var 0))
+
+@[simp]
+theorem wk_lift_pack0 {ℓ : ℕ} : (pack0 ℓ).wk (Nat.liftWk ρ) = pack0 (φ := φ) ℓ := by
+  simp only [pack0]
+  induction ℓ with
+  | zero => rfl
+  | succ ℓ ih => simp [ih, -Function.iterate_succ, Function.iterate_succ']
+
+@[simp]
+theorem wk1_pack0 : (pack0 ℓ).wk1 = pack0 (φ := φ) ℓ := by
+  simp only [wk1, wk_lift_pack0]
+
+@[simp]
+theorem subst_lift_pack0 {ℓ : ℕ} {σ : Subst φ} : (pack0 ℓ).subst σ.lift = pack0 (φ := φ) ℓ := by
+  simp only [pack0]
+  induction ℓ with
+  | zero => rfl
+  | succ ℓ ih => simp [ih, -Function.iterate_succ, Function.iterate_succ']
+
+@[simp]
+theorem Wf.pack0 {Γ : Ctx α ε} {R : LCtx α} {i : Fin R.length}
+  : Term.Wf (φ := φ) ((R.get i, ⊥)::Γ) (pack0 i) (R.pack, ⊥)  := by
+  induction R generalizing Γ with
+  | nil => exact i.elim0
+  | cons _ _ I =>
+    cases i using Fin.cases with
+    | zero => exact Wf.inl $ Wf.var Ctx.Var.shead
+    | succ i =>
+      simp only [Fin.val_succ,
+        BinSyntax.Term.pack0, Function.iterate_succ', Function.comp_apply, LCtx.pack, Wf.inr_iff]
+      apply I
+
+def InS.pack0 {Γ : Ctx α ε} (R : LCtx α) (i : Fin R.length)
+  : Term.InS φ ((R.get i, ⊥)::Γ) (R.pack, ⊥) :=
+  ⟨Term.pack0 i, Term.Wf.pack0⟩
+
+@[simp]
+theorem InS.coe_pack {Γ : Ctx α ε} {R : LCtx α} {i : Fin R.length}
+  : (InS.pack0 (φ := φ) (Γ := Γ) (R := R) i : Term φ) = Term.pack0 i := rfl
+
+@[simp]
+theorem InS.wk_lift_pack0 {Γ : Ctx α ε} {R : LCtx α} {i : Fin R.length} {ρ : Γ.InS Δ}
+  : (InS.pack0 (φ := φ) R i).wk (ρ.lift (le_refl _)) = pack0 R i := by ext; simp
+
+@[simp]
+theorem InS.wk_slift_pack0 {Γ : Ctx α ε} {R : LCtx α} {i : Fin R.length} {ρ : Γ.InS Δ}
+  : (InS.pack0 (φ := φ) R i).wk (ρ.slift) = pack0 R i := by ext; simp
+
+@[simp]
+theorem InS.subst_lift_pack0 {Γ : Ctx α ε} {R : LCtx α} {i : Fin R.length} {σ : Subst.InS φ Γ Δ}
+  : (InS.pack0 (φ := φ) R i).subst (σ.lift (le_refl _)) = pack0 R i := by ext; simp
+
+@[simp]
+theorem InS.subst_slift_pack0 {Γ : Ctx α ε} {R : LCtx α} {i : Fin R.length} {σ : Subst.InS φ Γ Δ}
+  : (InS.pack0 (φ := φ) R i).subst σ.slift = pack0 R i := by ext; simp
+
+@[simp]
+theorem InS.wk1_pack0 {Γ : Ctx α ε} {R : LCtx α} {i : Fin R.length}
+  : (InS.pack0 (φ := φ) (Γ := Γ) R i).wk1 (inserted := inserted) = pack0 R i := by ext; simp
+
+end Term
+
+namespace Region
+
+variable
+  [Φ: EffInstSet φ (Ty α) ε] [PartialOrder α] [PartialOrder ε] [OrderBot ε]
+  {Γ Δ : Ctx α ε} {σ : Region.Subst φ}
+
+open Term
+
+def Subst.pack : Region.Subst φ := λℓ => br 0 (Term.pack0 ℓ)
+
+@[simp]
+theorem Subst.Wf.pack {Γ : Ctx α ε} {R : LCtx α}
+  : Subst.Wf Γ R [R.pack] (Subst.pack (φ := φ)) := λ_ => Wf.br LCtx.Trg.shead Term.Wf.pack0
+
+@[simp]
+def Subst.InS.pack {Γ : Ctx α ε} {R : LCtx α} : Subst.InS φ Γ R [R.pack] :=
+  ⟨Subst.pack, Subst.Wf.pack⟩
+
+@[simp]
+theorem Subst.InS.coe_pack {Γ : Ctx α ε} {R : LCtx α} (ℓ : ℕ)
+  : (Subst.InS.pack (φ := φ) (Γ := Γ) (R := R) : Region.Subst φ) ℓ = br 0 (Term.pack0 ℓ) := rfl
+
+@[simp]
+theorem Subst.vlift_pack
+  : pack.vlift = pack (φ := φ) := by funext ℓ; simp [pack, Subst.vlift, vwk1]
+
+@[simp]
+theorem Subst.InS.vlift_pack {Γ : Ctx α ε} {R : LCtx α}
+  : (pack (φ := φ) (Γ := Γ) (R := R)).vlift (head := head) = pack := by ext; simp
+
+def unpack : ℕ → Region φ
+  | 0 => loop
+  | r + 1 => case (var 0) nil ((unpack r).lwk0)
+
+@[simp]
+theorem vwk_lift_unpack (r : ℕ) : (unpack r).vwk (Nat.liftWk ρ) = unpack (φ := φ) r := by
+  induction r generalizing ρ with
+  | zero => rw [unpack, vwk_loop]
+  | succ r ih =>
+    rw [unpack, vwk]
+    congr
+    rw [lwk0, vwk_lwk, ih]
+
+@[simp]
+theorem vwk1_unpack (r : ℕ) : (unpack r).vwk1 = unpack (φ := φ) r := by
+  rw [vwk1, vwk_lift_unpack]
+
+@[simp]
+theorem vsubst_lift_unpack {ρ : Term.Subst φ} (r : ℕ)
+  : (unpack r).vsubst ρ.lift = unpack (φ := φ) r := by
+  induction r generalizing ρ with
+  | zero => rw [unpack, vsubst_loop]
+  | succ r ih =>
+    rw [unpack, vsubst]
+    congr
+    rw [lwk0, vsubst_lwk, ih]
+
+@[simp]
+theorem Wf.unpack' {Γ : Ctx α ε} {R L : LCtx α}
+  : Wf ((R.pack, ⊥)::Γ) (unpack (φ := φ) R.length) (R ++ L) :=
+  by induction R generalizing Γ with
+  | nil => exact Wf.loop
+  | cons _ _ I => exact Wf.case (Term.Wf.var Ctx.Var.shead) Wf.nil I.lwk0
+
+@[simp]
+theorem Wf.unpack {Γ : Ctx α ε} {R : LCtx α}
+  : Wf ((R.pack, ⊥)::Γ) (unpack (φ := φ) R.length) R :=
+  by induction R generalizing Γ with
+  | nil => exact Wf.loop
+  | cons _ _ I => exact Wf.case (Term.Wf.var Ctx.Var.shead) Wf.nil I.lwk0
+
+@[simp]
+def InS.unpack {Γ : Ctx α ε} {R : LCtx α} : InS φ ((R.pack, ⊥)::Γ) R :=
+  ⟨Region.unpack R.length, Wf.unpack⟩
+
+@[simp]
+theorem InS.coe_unpack {Γ : Ctx α ε} {R : LCtx α}
+  : (InS.unpack (φ := φ) (Γ := Γ) (R := R) : Region φ) = Region.unpack R.length :=
+  rfl
+
+@[simp]
+theorem InS.vwk_lift_unpack {Γ : Ctx α ε} {R : LCtx α} {ρ : Γ.InS Δ}
+  : (InS.unpack (φ := φ) (R := R)).vwk (ρ.lift (le_refl _)) = unpack := by ext; simp
+
+@[simp]
+theorem InS.vwk1_unpack {Γ : Ctx α ε} {R : LCtx α}
+  : (InS.unpack (φ := φ) (Γ := Γ) (R := R)).vwk1 (inserted := inserted) = unpack := by ext; simp
+
+def Subst.InS.unpack {Γ : Ctx α ε} {R : LCtx α} : Subst.InS φ Γ [R.pack] R :=
+  Region.InS.unpack.csubst
+
+@[simp]
+theorem Subst.InS.coe_unpack {Γ : Ctx α ε} {R : LCtx α}
+  : (Subst.InS.unpack (φ := φ) (Γ := Γ) (R := R) : Region.Subst φ)
+  = Region.csubst (Region.unpack R.length) :=
+  rfl
+
+@[simp]
+theorem Subst.InS.vlift_unpack {Γ : Ctx α ε} {R : LCtx α} {ρ : Γ.InS Δ}
+  : (Subst.InS.unpack (φ := φ) (Γ := Γ) (R := R)).vlift (head := head) = unpack := by
+  ext; simp [Subst.vlift]
+
+open Term
+
+end Region
